theories/examples/list_new.v
@@ -595,7 +595,7 @@ Section list.
         rmap (* register map *)
         f_m b_m e_m (* malloc addrs *)
         b_r e_r a_r a_r' (* environment table addrs *)
-        ι ι1 ι2 γ Ep φ (* invariant/gname names *) :
+        ι ι1 γ Ep φ (* invariant/gname names *) :
 
     (* PC assumptions *)
     ExecPCPerm pc_p →
@@ -612,9 +612,8 @@ Section list.
     withinBounds (RW, b_r, e_r, a_r') = true →
     (a_r + f_m)%a = Some a_r' →
 
-    up_close (B:=coPset) ι1 ⊆ Ep →
-    up_close (B:=coPset) ι ⊆ Ep ∖ ↑ι1 →
-    up_close (B:=coPset) ι2 ⊆ Ep ∖ ↑ι1 ∖ ↑ι →
+    up_close (B:=coPset) ι ⊆ Ep →
+    up_close (B:=coPset) ι1 ⊆ Ep ∖ ↑ι →
 
     PC ↦ᵣ inr (pc_p,pc_b,pc_e,a_first)
        ∗ r_env ↦ᵣ inr (RWX,ll,ll',ll)
@@ -624,9 +623,9 @@ Section list.
        (* own token *)
        ∗ na_own logrel_nais Ep
        (* trusted code *)
-       ∗ na_inv logrel_nais ι1 (codefrag a_first (appendb_instr f_m))
+       ∗ codefrag a_first (appendb_instr f_m)
        (* malloc *)
-       ∗ na_inv logrel_nais ι2 (malloc_inv b_m e_m)
+       ∗ na_inv logrel_nais ι1 (malloc_inv b_m e_m)
        ∗ pc_b ↦ₐ inr (RO, b_r, e_r, a_r)
        ∗ a_r' ↦ₐ inr (E, b_m, e_m, b_m)
        (* linked list invariants *)
@@ -640,13 +639,13 @@ Section list.
           ∗ ([∗ map] r↦w ∈ <[r_t2:=inl 0%Z]> (<[r_t3:=inl 0%Z]> (<[r_t4:=inl 0%Z]>
                           (<[r_t5:=inl 0%Z]> (<[r_t6:=inl 0%Z]> rmap)))), r ↦ᵣ w)
           ∗ (∃ a a' pbvals', ⌜(a + 2 = Some a')%a⌝ ∗ prefLL γ (pbvals ++ pbvals' ++ [(a,w)]) ∗ r_t1 ↦ᵣ inr (RWX,a,a',a))
+          ∗ codefrag a_first (appendb_instr f_m)
           ∗ na_own logrel_nais Ep
           -∗ WP Seq (Instr Executable) {{ φ }})
       -∗
       WP Seq (Instr Executable) {{ λ v, φ v ∨ ⌜v = FailedV⌝ }}.
   Proof.
-    iIntros (Hvpc Hcont Hhd Hdom Hbounds Hf_m Hnclose Hnclose2 Hnclose3) "(HPC & Hr_env & Hr_t1 & Hr_t0 & Hregs & Hown & #Happ & #Hmalloc & Hpc_b & Ha_r' & #Hseal_inv & #Hpref & Hφ)".
-    iMod (na_inv_acc with "Happ Hown") as "(>Hprog & Hown & Hcls)";auto.
+    iIntros (Hvpc Hcont Hhd Hdom Hbounds Hf_m Hnclose Hnclose2) "(HPC & Hr_env & Hr_t1 & Hr_t0 & Hregs & Hown & Hprog & #Hmalloc & Hpc_b & Ha_r' & #Hseal_inv & #Hpref & Hφ)".
     iMod (na_inv_acc with "Hseal_inv Hown") as "(>HisList & Hown & Hcls')";[auto|solve_ndisj|].
     iDestruct "HisList" as (hd) "[Hll HisList]". iDestruct "HisList" as (pbvals') "(HisList & Hexact)".
     iDestruct (big_sepL2_length with "Hprog") as %Hprog_length.
@@ -717,9 +716,8 @@ Section list.
       iMod ("Hcls'" with "[HisList Hll Hexact $Hown]") as "Hown".
       { iNext. iExists _; iFrame. iExists _. iFrame. }
       unfocus_block "Hprog" "Hcont" as "Hprog".
-      iMod ("Hcls" with "[$Hprog $Hown]") as "Hown".
       iApply ("Hφ" with "[- $HPC $Hown $Hr_t0 $Hpc_b $Ha_r' $Hr_env]").
-      iSplitR "Hr_t1".
+      iSplitR "Hr_t1 Hprog".
       { iDestruct (big_sepM_insert with "[$Hregs $Hr_t3]") as "Hregs";[apply lookup_delete|rewrite insert_delete].
         repeat (rewrite -delete_insert_ne//).
         iDestruct (big_sepM_insert with "[$Hregs $Hr_t2]") as "Hregs";[apply lookup_delete|rewrite insert_delete -delete_insert_ne//].
@@ -728,7 +726,7 @@ Section list.
         repeat (rewrite -delete_insert_ne//). rewrite !(insert_commute _ _ r_env); auto.
         rewrite delete_insert. 2: rewrite !lookup_insert_ne// elem_of_gmap_dom_none Hdom;set_solver.
         rewrite - !(insert_commute _ r_t6)// - !(insert_commute _ r_t5)// - !(insert_commute _ r_t4)// - !(insert_commute _ r_t3)// - !(insert_commute _ r_t2)//. }
-      destruct Hpref.
+      destruct Hpref. iFrame "∗".
       iExists bnew,enew,x. rewrite H app_assoc. iFrame "Hpref' Hr_t1".
       auto. }
     { iInstr "Hprog". iGo "Hprog". solve_addr.
@@ -740,9 +738,8 @@ Section list.
       iMod ("Hcls'" with "[Hbnew Ha Hll Hexact $Hown]") as "Hown".
       { iNext. iExists _; iFrame. iExists [(bnew,w)]. iFrame. iExists _,_,_.
         repeat iSplit;eauto. iContiguous_next H1 0. }
-      iMod ("Hcls" with "[$Hprog $Hown]") as "Hown".
       iApply ("Hφ" with "[- $HPC $Hown $Hr_t0 $Hpc_b $Ha_r' $Hr_env]").
-      iSplitR "Hr_t1".
+      iFrame "∗". iSplitR "Hr_t1".
       { iDestruct (big_sepM_insert with "[$Hregs $Hr_t3]") as "Hregs";[apply lookup_delete|rewrite insert_delete].
         repeat (rewrite -delete_insert_ne//).
         iDestruct (big_sepM_insert with "[$Hregs $Hr_t2]") as "Hregs";[apply lookup_delete|rewrite insert_delete -delete_insert_ne//].
@@ -757,21 +754,43 @@ Section list.
   (* ------------------------------------------------------------------------------------------------- *)
   (* -------------------------------------------- FINDB ---------------------------------------------- *)
 
+  (* TODO: move this to the rules_Get.v file. small issue with the spec of failure: it does not actually
+     require/leave a trace on dst! It would be good if req_regs of a failing get does not include dst (if possible) *)
+  Lemma wp_Get_fail E get_i dst src pc_p pc_b pc_e pc_a w zsrc wdst :
+    decodeInstrW w = get_i →
+    is_Get get_i dst src →
+    isCorrectPC (inr (pc_p,pc_b,pc_e,pc_a)) →
+
+    {{{ ▷ PC ↦ᵣ inr (pc_p,pc_b,pc_e,pc_a)
+      ∗ ▷ pc_a ↦ₐ w
+      ∗ ▷ dst ↦ᵣ wdst
+      ∗ ▷ src ↦ᵣ inl zsrc }}}
+      Instr Executable @ E
+      {{{ RET FailedV; True }}}.
+  Proof.
+    iIntros (Hdecode Hinstr Hvpc φ) "(>HPC & >Hpc_a & >Hsrc & >Hdst) Hφ".
+    iDestruct (map_of_regs_3 with "HPC Hsrc Hdst") as "[Hmap (%&%&%)]".
+    iApply (wp_Get with "[$Hmap Hpc_a]"); eauto; simplify_map_eq; eauto.
+      by erewrite regs_of_is_Get; eauto; rewrite !dom_insert; set_solver+.
+    iNext. iIntros (regs' retv) "(#Hspec & Hpc_a & Hmap)". iDestruct "Hspec" as %Hspec.
+    destruct Hspec as [* Hsucc |].
+    { (* Success (contradiction) *) simplify_map_eq. }
+    { (* Failure, done *) by iApply "Hφ". }
+  Qed.
 
   (* The following describes a generalized spec for one arbitrary iteration of the find loop *)
   Lemma findb_spec_middle pc_p pc_b pc_e (* PC *)
         wret (* return cap *)
         b (* input z *)
-        findb_addrs (* program addresses *)
         ll pbvals hdw (* linked list head and pointers *)
-        a_first a_last (* special adresses *)
+        a_first (* special adresses *)
         E γ φ (* invariant/gname names *) :
 
     (* PC assumptions *)
-    isCorrectPC_range pc_p pc_b pc_e a_first a_last ->
+    ExecPCPerm pc_p →
 
     (* Program adresses assumptions *)
-    contiguous_between findb_addrs a_first a_last ->
+    SubBounds pc_b pc_e a_first (a_first ^+ length findb_instr)%a →
 
     (* linked list ptr element d *)
     hdw = inl 0%Z ∨ (∃ d d', hdw = inr (RWX,d,d',d) ∧ (d + 2)%a = Some d' ∧ d ∈ pbvals.*1) →
@@ -790,9 +809,9 @@ Section list.
       (* token which states all non atomic invariants are closed *)
       ∗ na_own logrel_nais E
       (* trusted code *)
-      ∗ findb_loop findb_addrs
+      ∗ codefrag a_first findb_instr
       ∗ ▷ φ FailedV
-      ∗ ▷ (findb_loop findb_addrs
+      ∗ ▷ (codefrag a_first findb_instr
           ∗ PC ↦ᵣ updatePcPerm wret
           ∗ r_t0 ↦ᵣ wret
           ∗ r_t2 ↦ᵣ inl 0%Z
@@ -807,10 +826,6 @@ Section list.
     iLöb as "IH" forall (pbvals hdw). (* we prove this spec by Löb induction for the case where we loop back *)
     iIntros (Hvpc Hcont Hd (* Hnclose *)) "(HPC & Hr_t0 & Hr_env & Hr_t1 & Hr_t2 & Hr_t3
     & Hseal_inv & Hown & Hprog & Hφfailed & Hφ)".
-    iDestruct (big_sepL2_length with "Hprog") as %Hprog_length.
-    destruct_list findb_addrs.
-    apply contiguous_between_cons_inv_first in Hcont as Heq. subst a.
-    (* get some general purpose registers *)
     iDestruct "Hr_t2" as (w2) "Hr_t2".
     iDestruct "Hr_t3" as (w3) "Hr_t3".
 
@@ -818,167 +833,69 @@ Section list.
        then the search has failed, and will crash with the getb instruction. *)
     destruct Hd as [-> | (d & d' & -> & Hd & Hin)].
     { (* getb r_t2 r_env: FAILED INSTRUCTION *)
-      iPrologue "Hprog".
-      iApply (wp_Get_fail with "[$HPC $Hi $Hr_t2 $Hr_env]");
-        [apply decode_encode_instrW_inv|eauto|iCorrectPC a_first a_last|..].
-      iEpilogue "_". iApply wp_value. iFrame. }
+      codefrag_facts "Hprog".
+      iInstr_lookup "Hprog" as "Hi" "Hcont".
+      wp_instr.
+      iApplyCapAuto @wp_Get_fail.
+      wp_pure. iApply wp_value. iFrame. }
 
     (* the successful case lets us load the b bound *)
-    (* getb r_t2 r_env *)
-    iPrologue "Hprog".
-    iApply (wp_Get_success with "[$HPC $Hi $Hr_t2 $Hr_env]");
-      [apply decode_encode_instrW_inv|auto|iCorrectPC a_first a_last|iContiguous_next Hcont 0|..].
-    iEpilogue "(HPC & Hprog_done & Hr_env & Hr_t2)". iSimpl in "Hr_t2".
-    (* sub r_t2 r_t2 r_t1 *)
-    iPrologue "Hprog".
-    iApply (wp_add_sub_lt_success_dst_r with "[$HPC $Hi $Hr_t1 $Hr_t2]");
-      [apply decode_encode_instrW_inv|auto|iContiguous_next Hcont 1|iCorrectPC a_first a_last|..].
-    iEpilogue "(HPC & Hi & Hr_t1 & Hr_t2)". iCombine "Hi" "Hprog_done" as "Hprog_done". iSimpl in "Hr_t2".
-    (* move r_t3 PC *)
-    iPrologue "Hprog".
-    iApply (wp_move_success_reg_fromPC with "[$HPC $Hi $Hr_t3]");
-      [apply decode_encode_instrW_inv|iCorrectPC a_first a_last|iContiguous_next Hcont 2|..].
-    iEpilogue "(HPC & Hi & Hr_t3)". iCombine "Hi" "Hprog_done" as "Hprog_done".
-    (* lea r_t3 6 *)
-    assert (a1 + 6 = Some a7)%a as Hlea.
-    { apply contiguous_between_incr_addr_middle with (i:=2) (j:=6) (ai:=a1) (aj:=a7) in Hcont;auto. }
-    iPrologue "Hprog".
-    iApply (wp_lea_success_z with "[$HPC $Hi $Hr_t3]");
-      [apply decode_encode_instrW_inv|iCorrectPC a_first a_last|iContiguous_next Hcont 3|apply Hlea|..].
-    { eapply isCorrectPC_range_perm_non_E;eauto. apply contiguous_between_length in Hcont. clear -Hcont. solve_addr. }
-    iEpilogue "(HPC & Hi & Hr_t3)". iCombine "Hi" "Hprog_done" as "Hprog_done".
-
+    codefrag_facts "Hprog".
+    do 4 iInstr "Hprog". (* Can't use iGo as we need to do a case analysis. *)
     (* again we branch in two different cases: either the current word is the
        one we are searching for, and we will return to r_t0, or we must get the next pointer
        and start over *)
 
     destruct (decide (d - b = 0)%Z).
     { rewrite e.
-      (* jnz r_t3 r_t2 *)
-      iPrologue "Hprog".
-      iApply (wp_jnz_success_next with "[$HPC $Hi $Hr_t3 $Hr_t2]");
-        [apply decode_encode_instrW_inv|iCorrectPC a_first a_last|iContiguous_next Hcont 4|..].
-      iEpilogue "(HPC & Hi & Hr_t3 & Hr_t2)"; iCombine "Hi" "Hprog_done" as "Hprog_done".
-      (* load r_t1 r_env *)
-      (* iMod (na_inv_open with "Hseal_inv Hown") as "(>Hlist & Hown & Hcls)";[auto|solve_ndisj|]. *)
       iDestruct "Hseal_inv" as (hd) "[Hll Hlist]". iDestruct "Hlist" as "[HisList Hexact]".
       apply elem_of_list_fmap in Hin as [ [dp dw] [Heq Hin] ]. simpl in Heq; subst dp.
       iDestruct (isList_extract _ _ d with "HisList") as (a' hd' Hcond) "[Ha [Ha' Hcls'] ]"; eauto.
-      iPrologue "Hprog".
-      iApply (wp_load_success_alt with "[$HPC $Hi $Hr_t1 $Hr_env $Ha]");
-        [apply decode_encode_instrW_inv|iCorrectPC a_first a_last| |iContiguous_next Hcont 5|..].
-      { split;auto. apply andb_true_iff. rewrite Z.leb_le Z.ltb_lt. revert Hd;clear;solve_addr. }
-      iEpilogue "(HPC & Hr_t1 & Hi & Hr_env & Hd)"; iCombine "Hi" "Hprog_done" as "Hprog_done".
-      iDestruct ("Hcls'" with "[$Hd $Ha']") as "HisList".
-      (* iMod ("Hcls" with "[HisList Hll Hexact $Hown]") as "Hown";[iNext;iExists _;iFrame;iExists _;iFrame|].  *)
-      (* move r_t3 0 *)
-      iPrologue "Hprog".
-      iApply (wp_move_success_z with "[$HPC $Hi $Hr_t3]");
-        [apply decode_encode_instrW_inv|iCorrectPC a_first a_last|iContiguous_next Hcont 6|..].
-      iEpilogue "(HPC & Hi & Hr_t3)"; iCombine "Hi" "Hprog_done" as "Hprog_done".
-      (* jmp r_t0 *)
-      iPrologue "Hprog".
-      iApply (wp_jmp_success with "[$HPC $Hi $Hr_t0]");
-        [apply decode_encode_instrW_inv|iCorrectPC a_first a_last|..].
-      iEpilogue "(HPC & Hi & Hr_t0)"; iCombine "Hi" "Hprog_done" as "Hprog_done".
-      (* continuation *)
-      iApply "Hφ".
-      iSplitL "Hprog Hprog_done".
-      { iFrame. iDestruct "Hprog_done" as "($&$&$&$&$&$&$&$&$)". }
-      iFrame. iSplitR "Hll HisList";[|iExists _;iFrame]. iExists d,d',_. iFrame. iSplit;auto.
-      iPureIntro. assert (z_of d = b)%Z as <-;[clear -e;lia|]. apply z_to_addr_z_of.
-    }
+      iGo "Hprog". split; [auto|solve_addr].
+      iGo "Hprog".
+      iApply "Hφ". iFrame.
+      iDestruct ("Hcls'" with "[$Ha $Ha']") as "HisList".
+      iSplitR "Hll HisList";[|iExists _;iFrame]. iExists d,d',_. iFrame. iSplit;auto.
+      iPureIntro. assert (z_of d = b)%Z as <-;[clear -e;lia|]. apply z_to_addr_z_of. }
 
-    (* jnz r_t3 r_t2 *)
-    iPrologue "Hprog".
-    iApply (wp_jnz_success_jmp with "[$HPC $Hi $Hr_t3 $Hr_t2]");
-      [apply decode_encode_instrW_inv|iCorrectPC a_first a_last|..].
-    { intros Hcontr. inversion Hcontr. done. }
-    iEpilogue "(HPC & Hi & Hr_t3 & Hr_t2)"; iCombine "Hi" "Hprog_done" as "Hprog_done".
-    (* skip the instructions we jumped over *)
-    do 3 (iDestruct "Hprog" as "[Hi Hprog]";iCombine "Hi" "Hprog_done" as "Hprog_done").
-    assert (updatePcPerm (inr (pc_p, pc_b, pc_e, a7)) = (inr (pc_p, pc_b, pc_e, a7))) as ->.
-    { apply isCorrectPC_range_perm_non_E in Hvpc;[|apply contiguous_between_length in Hcont;
-                                                   simpl in Hcont;clear -Hcont;solve_addr].
-      destruct pc_p;auto. done. }
-    (* lea r_env 1 *)
-    assert (is_Some (d + 1)%a) as [d'' Hd''].
-    { destruct (d + 1)%a eqn:Hcontr;eauto. clear -Hcontr Hd; solve_addr. }
-    iPrologue "Hprog".
-    iApply (wp_lea_success_z with "[$HPC $Hi $Hr_env]");
-      [apply decode_encode_instrW_inv|iCorrectPC a_first a_last|iContiguous_next Hcont 8|apply Hd''|auto|].
-    iEpilogue "(HPC & Hi & Hr_env)". iCombine "Hi" "Hprog_done" as "Hprog_done".
-    (* load r_env r_env *)
-    iPrologue "Hprog".
-    (* iMod (na_inv_open with "Hseal_inv Hown") as "(Hlist & Hown & Hcls')";[auto|solve_ndisj|].  *)
+    iGo "Hprog". congruence.
+    generalize (updatePcPerm_cap_non_E pc_p pc_b pc_e (a_first ^+ 8)%a ltac:(destruct Hvpc; congruence)); rewrite /updatePcPerm; intros HX; rewrite HX; clear HX.
     iDestruct "Hseal_inv" as (hd) "[Hll Hlist]".
     iDestruct "Hlist" as "[Hlist Hexact]".
-    (* iDestruct (isList_NoDup with "Hlist") as %Hdup. *)
-    (* assert (list.last (hd::ptrs'') ≠ Some d) as Hn.  *)
-    (* { apply rest_last with (l1:=hd::ptrs) (l2:=hd::ptrs');eauto;apply prefix_cons;auto. } *)
     apply elem_of_list_fmap in Hin as [ [dp dw] [Heq Hin] ]. simpl in Heq; subst dp.
     iDestruct (isList_extract _ _ d with "Hlist") as (a' hd' (Hincr&Hcond)) "(Ha1 & Ha2 & Hcls'')";eauto.
     simplify_eq.
-    iApply (wp_load_success_same_alt with "[$HPC $Hi $Hr_env $Ha2]");
-      [apply decode_encode_instrW_inv|iCorrectPC a_first a_last| |iContiguous_next Hcont 9|..].
-    { split;auto. apply andb_true_iff. rewrite Z.leb_le Z.ltb_lt. revert Hd Hd'';clear;solve_addr. }
-    iNext. iIntros "(HPC & Hr_env & Hi & Ha2)". iCombine "Hi" "Hprog_done" as "Hprog_done".
+    iGo "Hprog". solve_addr.
     iMod (get_full_pref with "Hexact") as "[Hexact #Hpref'']".
     iDestruct ("Hcls''" with "[$Ha1 $Ha2]") as "Hlist".
-    (* iMod ("Hcls'" with "[Hexact Hlist Hll $Hown]") as "Hown";[iNext;iExists _;iFrame;iExists _;iFrame|].  *)
-    iApply wp_pure_step_later;auto;iNext.
-    (* move r_t2 PC *)
-    iPrologue "Hprog".
-    iApply (wp_move_success_reg_fromPC with "[$HPC $Hi $Hr_t2]");
-      [apply decode_encode_instrW_inv|iCorrectPC a_first a_last|iContiguous_next Hcont 10|..].
-    iEpilogue "(HPC & Hi & Hr_t2)"; iCombine "Hi" "Hprog_done" as "Hprog_done".
-    (* lea r_t2 -11 *)
-    assert (a9 + (-10) = Some a_first)%a as Hlea'.
-    { apply contiguous_between_incr_addr_middle with (i:=0) (j:=10) (ai:=a_first) (aj:=a9) in Hcont;auto. clear -Hcont; solve_addr. }
-    iPrologue "Hprog".
-    iApply (wp_lea_success_z with "[$HPC $Hi $Hr_t2]");
-      [apply decode_encode_instrW_inv|iCorrectPC a_first a_last|iContiguous_next Hcont 11|apply Hlea'|..].
-    { apply isCorrectPC_range_perm_non_E in Hvpc;auto.
-      apply contiguous_between_length in Hcont. clear-Hcont. solve_addr. }
-    iEpilogue "(HPC & Hi & Hr_t2)"; iCombine "Hi" "Hprog_done" as "Hprog_done".
-    (* jmp r_t2 *)
-    iPrologue "Hprog".
-    iApply (wp_jmp_success with "[$HPC $Hi $Hr_t2]");
-      [apply decode_encode_instrW_inv|iCorrectPC a_first a_last|..].
-    iEpilogue "(HPC & Hi & Hr_t2)"; iCombine "Hi" "Hprog_done" as "Hprog_done".
-    (* apply IH since we have looped back *)
-    assert (updatePcPerm (inr (pc_p, pc_b, pc_e, a_first)) = inr (pc_p, pc_b, pc_e, a_first)) as ->.
-    { apply isCorrectPC_range_perm_non_E in Hvpc. destruct pc_p;auto. done.
-      apply contiguous_between_length in Hcont. clear-Hcont. solve_addr. }
-
-    iApply ("IH" with "[] [] [] [$HPC $Hr_env $Hr_t0 $Hr_t1 $Hφ $Hφfailed Hprog_done Hexact Hlist Hll Hr_t2 Hr_t3 $Hown]");auto.
+    iGo "Hprog". instantiate (1 := a_first). solve_addr.
+    iInstr "Hprog". generalize (updatePcPerm_cap_non_E pc_p pc_b pc_e (a_first)%a ltac:(destruct Hvpc; congruence)); rewrite /updatePcPerm; intros HX; rewrite HX; clear HX.
+    iApply ("IH" with "[] [] [] [$HPC $Hr_env $Hr_t0 $Hr_t1 $Hφ $Hφfailed $Hprog Hexact Hlist Hll Hr_t2 Hr_t3 $Hown]");auto.
     { iPureIntro. destruct Hcond as [ (-> & _) | (p & p' & w' & Hp & -> & Hin') ];[by left|right].
       repeat eexists;auto. apply elem_of_list_fmap. exists (p,w'). eauto. }
     iSplitL "Hr_t2";[eauto|]. iSplitL "Hr_t3";eauto.
-    iDestruct "Hprog_done" as "($&$&$&$&$&$&$&$&$&$&$&$&$&$)". iSplitL;[|done].
     iExists hd. iFrame.
   Qed.
 
   (* The following describes the spec for the full program, starting at the first node of the LL *)
-  (* The list of knows prefixes is arbitrary, since the proof builds up known prefixes as it goes along *)
+  (* The list of known prefixes is arbitrary, since the proof builds up known prefixes as it goes along *)
   Lemma findb_spec pc_p pc_b pc_e (* PC *)
         wret (* return cap *)
         b (* input z *)
-        findb_addrs (* program addresses *)
         ll ll' (* linked list head and pointers *)
-        a_first a_last (* special adresses *)
-        ι ι1 γ φ (* invariant/gname names *) :
+        a_first (* special adresses *)
+        ι γ φ Ep (* invariant/gname names *) :
 
     (* PC assumptions *)
-    isCorrectPC_range pc_p pc_b pc_e a_first a_last ->
+    ExecPCPerm pc_p →
 
     (* Program adresses assumptions *)
-    contiguous_between findb_addrs a_first a_last ->
+    SubBounds pc_b pc_e a_first (a_first ^+ S (length findb_instr))%a →
 
     (* linked list ptr element d *)
     (ll + 1)%a = Some ll' →
 
-    up_close (B:=coPset) ι ⊆ ⊤ ∖ ↑ι1 →
+    up_close (B:=coPset) ι ⊆ Ep →
 
     PC ↦ᵣ inr (pc_p,pc_b,pc_e,a_first)
       ∗ r_t0 ↦ᵣ wret
@@ -989,50 +906,44 @@ Section list.
       (* invariant for d *)
       ∗ sealLL ι ll γ
       (* token which states all non atomic invariants are closed *)
-      ∗ na_own logrel_nais ⊤
+      ∗ na_own logrel_nais Ep
       (* trusted code *)
-      ∗ na_inv logrel_nais ι1 (findb findb_addrs)
+      ∗ codefrag a_first ((encodeInstrsW [Load r_env r_env])++findb_instr)
       ∗ ▷ φ FailedV
       ∗ ▷ (PC ↦ᵣ updatePcPerm wret
           ∗ r_t0 ↦ᵣ wret
           ∗ r_t2 ↦ᵣ inl 0%Z
           ∗ (∃ b_a b' w pbvals, ⌜z_to_addr b = Some b_a ∧ (b_a + 2)%a = Some b' ∧ (b_a,w) ∈ pbvals⌝ ∗ prefLL γ pbvals ∗ r_t1 ↦ᵣ w ∗ r_env ↦ᵣ inr (RWX,b_a,b',b_a))
           ∗ r_t3 ↦ᵣ inl 0%Z
-          ∗ na_own logrel_nais ⊤
+          ∗ codefrag a_first ((encodeInstrsW [Load r_env r_env])++findb_instr)
+          ∗ na_own logrel_nais Ep
           -∗ WP Seq (Instr Executable) {{ φ }})
       -∗
       WP Seq (Instr Executable) {{ φ }}.
   Proof.
     iIntros (Hvpc Hcont Hd Hnclose) "(HPC & Hr_t0 & Hr_env & Hr_t1 & Hr_t2 & Hr_t3
-    & #Hseal_inv & Hown & #Hfindb & Hφfailed & Hφ)".
-    iMod (na_inv_acc with "Hfindb Hown") as "(>Hprog & Hown & Hcls)";auto.
+    & #Hseal_inv & Hown & Hprog & Hφfailed & Hφ)".
     iDestruct (big_sepL2_length with "Hprog") as %Hprog_length.
     iMod (na_inv_acc with "Hseal_inv Hown") as "(>HisList & Hown & Hcls')";auto.
     iDestruct "HisList" as (hd) "[Hll HisList]". iDestruct "HisList" as (pbvals') "[HisList Hexact]".
     iDestruct (isList_hd_pure with "HisList") as %Hhd.
     iMod (get_full_pref with "Hexact") as "[Hexact #Hpref']".
-    (* load r_env r_env *)
-    destruct findb_addrs;[inversion Hprog_length|]. apply contiguous_between_cons_inv_first in Hcont as Heq;subst a.
-    destruct findb_addrs;[inversion Hprog_length|].
-    iPrologue "Hprog".
-    iApply (wp_load_success_same_alt with "[$HPC $Hi $Hr_env $Hll]");
-      [apply decode_encode_instrW_inv|iCorrectPC a_first a_last| |iContiguous_next Hcont 0|..].
-    { split;auto. apply andb_true_iff. rewrite Z.leb_le Z.ltb_lt. revert Hd;clear;solve_addr. }
-    iEpilogue "(HPC & Hr_env & Hi & Hll)".
-    apply contiguous_between_cons_inv in Hcont as [? [? [? Hcont] ] ];
-      apply contiguous_between_cons_inv_first in Hcont as ?;subst.
+
+    codefrag_facts "Hprog".
+    iInstr "Hprog". solve_addr.
+    focus_block 1 "Hprog" as a_middle Ha_middle "Hprog" "Hcont".
+    cbn in Ha_middle. replace a_middle with (a_first ^+ 1)%a by solve_addr.
     iApply (findb_spec_middle with "[-]");[..|iFrame "∗ #"];eauto.
-    { intros mid [Hmid Hmid']. apply isCorrectPC_inrange with a_first a_last; auto. split;auto.
-      trans x;auto. clear -H0;solve_addr. }
+    { solve_addr+ H0. }
     { destruct Hhd as [ (->&_) | (?&?&?&?&->&?) ];auto. right.
-      repeat eexists;auto. apply elem_of_list_fmap. exists (x0,x2). eauto. }
+      repeat eexists;auto. apply elem_of_list_fmap. exists (x,x1). eauto. }
     iSplitL "Hll HisList". iExists _;iFrame.
     iNext. iIntros "(Hprog & HPC & Hr_t0 & Hr_t2 & Hres & Hr_t3 & Hna & Hlist)".
     iDestruct "Hres" as (b_a b' w (Heq&Hincr&Hin)) "[Hr_t1 Hr_env]".
     iMod ("Hcls'" with "[Hlist $Hna]") as "Hown".
     { iNext. iDestruct "Hlist" as (hd') "[? [? ?] ]".
       iExists _; iFrame. iExists _; iFrame. }
-    iMod ("Hcls" with "[$Hi $Hprog $Hown]") as "Hown".
+    unfocus_block "Hprog" "Hcont" as "Hprog".
     iApply "Hφ". iFrame. iExists _,_,_,_. iFrame "∗ #". auto.
   Qed.
 
